Experimental requirements for rsloan-phoas

src/Assembly/QhasmUtil.v
@@ -1,50 +1,48 @@
-Require Import Coq.ZArith.ZArith Coq.NArith.NArith Coq.Numbers.Natural.Peano.NPeano.
-Require Import Crypto.Assembly.QhasmCommon.
-Require Import Crypto.Util.Notations.
-Require Export Bedrock.Word.
-Require Export Crypto.Util.FixCoqMistakes.
+Require Import ZArith NArith NPeano.
+Require Import QhasmCommon.
+Require Export Bedrock.Word Bedrock.Nomega.
 
 Delimit Scope nword_scope with w.
 Local Open Scope nword_scope.
 
-Notation "& x" := (wordToN x) : nword_scope.
-Notation "** x" := (NToWord _ x) : nword_scope.
+Notation "& x" := (wordToN x) (at level 30) : nword_scope.
+Notation "** x" := (NToWord _ x) (at level 30) : nword_scope.
 
 Section Util.
-  Definition convS {A B: Set} (x: A) (H: A = B) : B :=
-    eq_rect A (fun B0 : Set => B0) x B H.
-
-  Definition high {k n: nat} (p: (k <= n)%nat) (w: word n) : word k.
-    refine (split1 k (n - k) (convS w _)).
-    abstract (replace n with (k + (n - k)) by omega; intuition auto with arith).
+  Definition convS {n m} (x: word n) (H: n = m): word m.
+    refine (eq_rect _ (fun B0 : Set => B0) x _ _).
+    abstract (subst; intuition).
   Defined.
 
-  Definition low {k n: nat} (p: (k <= n)%nat) (w: word n) : word k.
-    refine (split2 (n - k) k (convS w _)).
-    abstract (replace n with (k + (n - k)) by omega; intuition auto with zarith).
+  Definition low {k n: nat} (p: (k <= n)%nat) (w: word n): word k.
+    refine (split1 k (n - k) (convS w _)); abstract omega.
   Defined.
 
-  Definition extend {k n: nat} (p: (k <= n)%nat) (w: word k) : word n.
-    refine (convS (zext w (n - k)) _).
-    abstract (replace (k + (n - k)) with n by omega; intuition).
+  Definition high {k n: nat} (p: (k <= n)%nat) (w: word n): word (n - k).
+    refine (split2 k (n - k) (convS w _)); abstract omega.
   Defined.
 
-  Definition shiftr {n} (w: word n) (k: nat) : word n :=
-    match (le_dec k n) with
-    | left p => extend p (high p w)
+  Definition extend {k n: nat} (p: (k <= n)%nat) (w: word k): word n.
+    refine (convS (zext w (n - k)) _); abstract omega.
+  Defined.
+
+  Definition shiftr {n} (w: word n) (k: nat): word n.
+    refine match (le_dec k n) with
+    | left p => extend _ (@high k _ _ w)
     | right _ => wzero n
-    end.
+    end; abstract nomega.
+  Defined.
 
-  Definition mask {n} (k: nat) (w: word n) : word n :=
+  Definition mask {n} (k: nat) (w: word n): word n :=
     match (le_dec k n) with
     | left p => extend p (low p w)
     | right _ => w
     end.
 
-  Definition overflows (n: nat) (x: N) :
-      {(x >= Npow2 n)%N} + {(x < Npow2 n)%N}.
+  Definition Nge_dec (x y: N) :
+      {(x >= y)%N} + {(x < y)%N}.
     refine (
-      let c := (x ?= Npow2 n)%N in
+      let c := (x ?= y)%N in
       match c as c' return c = c' -> _ with
       | Lt => fun _ => right _
       | _ => fun _ => left _
@@ -59,22 +57,26 @@ Section Util.
         end).
   Defined.
 
-  Definition break {n} (m: nat) (x: word n) : word m * word (n - m).
-    refine match (le_dec m n) with
-    | left p => (extend _ (low p x), extend _ (@high (n - m) n _ x))
-    | right p => (extend _ x, _)
-    end; try abstract intuition auto with zarith.
+  Definition overflows (n: nat) (x: N) := Nge_dec x (Npow2 n).
 
-    replace (n - m) with O by abstract omega; exact WO.
+  Definition ind (b: bool): N := if b then 1%N else 0%N.
+
+  Definition ind' {A B} (b: {A} + {B}): N := if b then 1%N else 0%N.
+
+  Definition break {n} (m: nat) (x: word n): word m * word (n - m).
+    refine match (le_dec m n) with
+    | left p => (extend _ (low p x), extend _ (@high m n _ x))
+    | right p => (extend _ x, extend _ WO)
+    end; try abstract intuition.
   Defined.
 
-  Definition addWithCarry {n} (x y: word n) (c: bool) : word n :=
+  Definition addWithCarry {n} (x y: word n) (c: bool): word n :=
     x ^+ y ^+ (natToWord _ (if c then 1 else 0)).
 
   Definition omap {A B} (x: option A) (f: A -> option B) :=
     match x with | Some y => f y | _ => None end.
 
-  Notation "A <- X ; B" := (omap X (fun A => B)).
+  Notation "A <- X ; B" := (omap X (fun A => B)) (at level 70, right associativity).
 End Util.
 
 Close Scope nword_scope.
