src/Assembly/Bounds.v
@@ -1,0 +1,426 @@
+Require Export Bedrock.Word Bedrock.Nomega.
+Require Import NArith PArith Ndigits Nnat NPow NPeano Ndec Ndigits.
+Require Import Compare_dec Omega.
+Require Import FunctionalExtensionality ProofIrrelevance.
+Require Import Crypto.Assembly.QhasmUtil Crypto.Assembly.QhasmEvalCommon Crypto.Assembly.WordizeUtil.
+
+Import EvalUtil.
+
+Hint Rewrite wordToN_nat Nat2N.inj_add N2Nat.inj_add
+             Nat2N.inj_mul N2Nat.inj_mul Npow2_nat : N.
+
+Open Scope nword_scope.
+
+Section Bounds.
+  Lemma wordize_plus': forall {n} (x y: word n) (b: N),
+      (&x < b)%N
+    -> (&y < (Npow2 n - b))%N
+    -> (b <= Npow2 n)%N
+    -> (&x + &y)%N = & (x ^+ y).
+  Proof.
+    intros.
+    unfold wplus, wordBin.
+    rewrite wordToN_NToWord; intuition.
+    apply (N.lt_le_trans _ (b + &y)%N _).
+
+    - apply N.add_lt_le_mono; try assumption.
+      apply N.eq_le_incl; reflexivity.
+
+    - replace (Npow2 n) with (b + Npow2 n - b)%N by nomega;
+        replace (b + Npow2 n - b)%N with (b + (Npow2 n - b))%N by (
+        replace (b + (Npow2 n - b))%N with ((Npow2 n - b) + b)%N by nomega;
+        rewrite (N.sub_add b (Npow2 n)) by assumption;
+        nomega).
+
+        apply N.add_le_mono_l; try nomega.
+        apply N.lt_le_incl; assumption.
+  Qed.
+
+  Lemma wordize_mult': forall {n} (x y: word n) (b: N),
+      (1 < n)%nat -> (0 < b)%N
+    -> (&x < b)%N
+    -> (&y < (Npow2 n) / b)%N
+    -> (&x * &y)%N = & (x ^* y).
+  Proof.
+    intros; unfold wmult, wordBin.
+    rewrite wordToN_NToWord; intuition.
+    apply (N.lt_le_trans _ (b * ((Npow2 n) / b))%N _).
+
+    - apply N.mul_lt_mono; assumption.
+
+    - apply N.mul_div_le; nomega.
+  Qed.
+
+  Lemma constant_bound_N : forall {n} (k: word n),
+    (& k < & k + 1)%N.
+  Proof. intros; nomega. Qed.
+
+  Lemma constant_bound_nat : forall (n k: nat),
+      (N.of_nat k < Npow2 n)%N
+    -> (& (@natToWord n k) < (N.of_nat k) + 1)%N.
+  Proof.
+    intros.
+    rewrite wordToN_nat.
+    rewrite wordToNat_natToWord_idempotent;
+      try assumption; nomega.
+  Qed.
+
+  Lemma let_bound : forall {n} (x: word n) (f: word n -> word n) xb fb,
+      (& x < xb)%N
+    -> (forall x', & x' < xb -> & (f x') < fb)%N
+    -> ((let k := x in &(f k)) < fb)%N.
+  Proof. intros; eauto. Qed.
+
+  Definition Nlt_dec (x y: N): {(x < y)%N} + {(x >= y)%N}.
+    refine (
+      let c := N.compare x y in
+      match c as c' return c = c' -> _ with
+      | Lt => fun _ => left _
+      | _ => fun _ => right _
+      end eq_refl);
+    abstract (
+      unfold c, N.ge, N.lt in *; intuition; subst;
+      match goal with
+      | [H0: ?x = _, H1: ?x = _ |- _] =>
+        rewrite H0 in H1; inversion H1
+      end).
+  Defined.
+
+  Lemma wplus_bound : forall {n} (w1 w2 : word n) b1 b2,
+      (&w1 < b1)%N
+    -> (&w2 < b2)%N
+    -> (&(w1 ^+ w2) < b1 + b2)%N.
+  Proof.
+    intros.
+
+    destruct (Nlt_dec (b1 + b2)%N (Npow2 n)) as [g|g].
+
+    - rewrite <- wordize_plus' with (b := b1);
+        try apply N.add_lt_mono;
+        try assumption.
+
+      + apply (N.lt_le_trans _ b2 _); try assumption.
+        apply N.lt_le_incl.
+        apply N.lt_add_lt_sub_l.
+        assumption.
+
+      + apply N.lt_le_incl; nomega.
+
+    - apply (N.lt_le_trans _ (Npow2 n) _).
+
+      + apply word_size_bound.
+
+      + unfold N.le, N.ge in *.
+        intro Hg.
+        contradict g.
+        rewrite N.compare_antisym.
+        rewrite Hg.
+        simpl; intuition.
+  Qed.
+
+  Theorem wmult_bound : forall {n} (w1 w2 : word n) b1 b2,
+      (1 < n)%nat
+    -> (&w1 < b1)%N
+    -> (&w2 < b2)%N
+    -> (&(w1 ^* w2) < b1 * b2)%N.
+  Proof.
+    intros.
+    destruct (Nlt_dec (b1 * b2)%N (Npow2 n)) as [g|g].
+
+    - rewrite <- wordize_mult' with (b := b1);
+        try apply N.mul_lt_mono;
+        try assumption;
+        try nomega.
+
+      apply (N.lt_le_trans _ b2 _); try assumption.
+      apply N.div_le_lower_bound.
+
+      + induction (& w1); nomega.
+
+      + apply N.lt_le_incl.
+        assumption.
+
+    - apply (N.lt_le_trans _ (Npow2 n) _).
+
+      + apply word_size_bound.
+
+      + unfold N.le, N.ge in *.
+        intro Hg.
+        contradict g.
+        rewrite N.compare_antisym.
+        rewrite Hg.
+        simpl; intuition.
+  Qed.
+
+  Lemma shiftr_bound : forall {n} (w : word n) b bits,
+      (&w < b)%N
+    -> (&(shiftr w bits) < N.succ (N.shiftr_nat b bits))%N.
+  Proof.
+    intros.
+    apply (N.le_lt_trans _ (N.shiftr_nat b bits) _).
+
+    - unfold shiftr, extend, high.
+      destruct (le_dec bits n); try omega.
+
+      + rewrite wordToN_convS.
+        rewrite wordToN_zext.
+        rewrite wordToN_split2.
+        rewrite wordToN_convS.
+        rewrite <- Nshiftr_equiv_nat.
+        repeat rewrite N.shiftr_div_pow2.
+        apply N.div_le_mono.
+
+        * induction bits; try nomega.
+          rewrite Nat2N.inj_succ.
+          rewrite N.pow_succ_r'.
+          assert (bits <= n)%nat as Hc by omega.
+          apply IHbits in Hc.
+          intro Hc'; contradict Hc.
+          apply (N.mul_cancel_l _ _ 2);
+            try rewrite Hc';
+            try assumption;
+            nomega.
+
+        * apply N.lt_le_incl.
+          assumption.
+
+      + rewrite wordToN_nat.
+        unfold wzero.
+        rewrite wordToNat_natToWord_idempotent; simpl;
+          try apply N_ge_0;
+          try apply Npow2_gt0.
+
+    - nomega.
+
+  Qed.
+
+  Lemma mask_bound : forall {n} (w : word n) m,
+    (&(mask m w) < Npow2 m)%N.
+  Proof.
+    intros.
+    unfold mask in *; destruct (le_dec m n); simpl;
+      try apply extend_bound.
+
+    pose proof (word_size_bound w) as H.
+    apply (N.le_lt_trans _ (Npow2 n) _).
+
+    - unfold N.le, N.lt in *; rewrite H; intro H0; inversion H0.
+
+    - clear H.
+      replace m with ((m - n) + n) by nomega.
+      replace (Npow2 n) with (1 * (Npow2 n))%N
+        by (rewrite N.mul_comm; nomega).
+      rewrite Npow2_split.
+      apply N.mul_lt_mono_pos_r; try apply Npow2_gt0.
+      assert (0 < m - n)%nat by omega.
+      induction (m - n); try inversion H; try abstract (
+        simpl; replace 2 with (S 1) by omega;
+        apply N.lt_1_2); subst.
+
+      assert (0 < n1)%nat as Z by omega; apply IHn1 in Z.
+      apply (N.le_lt_trans _ (Npow2 n1) _).
+
+      + apply N.lt_le_incl; assumption.
+
+      + rewrite Npow2_succ.
+        replace' (Npow2 n1) with (1 * Npow2 n1)%N at 1 by (apply N.mul_1_l).
+        apply N.mul_lt_mono_pos_r; try abstract (vm_compute; reflexivity).
+        apply (N.lt_le_trans _ 1 _); try abstract (vm_compute; reflexivity).
+        apply N.lt_le_incl; assumption.
+  Qed.
+
+  Lemma mask_update_bound : forall {n} (w : word n) b m,
+      (1 < n)%nat
+    -> (&w < b)%N
+    -> (&(mask m w) < (N.min b (Npow2 m)))%N.
+  Proof.
+    intros.
+    assert (& w mod Npow2 m < b)%N. {
+      destruct (Nge_dec (&w) (Npow2 m)).
+
+      - apply (N.lt_le_trans _ (Npow2 m) _).
+
+        + pose proof (N.mod_bound_pos (&w) (Npow2 m)
+                     (N_ge_0 _) (Npow2_gt0 _)) as H1.
+          destruct H1.
+          assumption.
+
+        + transitivity (&w); try abstract (apply ge_to_le; assumption).
+          apply N.lt_le_incl; assumption.
+
+      - rewrite N.mod_small; assumption.
+    }
+
+    unfold mask, N.min, extend, low;
+      destruct (le_dec m n),
+               (N.compare b (Npow2 m)); simpl;
+      repeat first [
+        rewrite wordToN_convS  |
+        rewrite wordToN_zext   |
+        rewrite wordToN_wones  |
+        rewrite wordToN_split1 |
+        rewrite N.land_ones    |
+        rewrite <- Npow2_N ];
+      try assumption.
+
+    - pose proof (N.mod_bound_pos (&w) (Npow2 m) (N_ge_0 _) (Npow2_gt0 _)) as Z.
+      destruct Z.
+      assumption.
+
+    - apply (N.lt_le_trans _ (Npow2 n) _);
+        try apply word_size_bound.
+      apply Npow2_ordered.
+      omega.
+  Qed.
+
+  Lemma plus_overflow_bound: forall x y a b,
+      (x < a)%N
+    -> (y < b - a)%N
+    -> (x + y < b)%N.
+  Proof. intros; nomega. Qed.
+
+End Bounds.
+
+(** Constant Tactics **)
+
+Ltac assert_nat_constant t :=
+  timeout 1 (match (eval vm_compute in t) with
+  | O => idtac
+  | S ?n => assert_nat_constant n
+  | _ => fail
+  end).
+
+Ltac assert_pos_constant t :=
+  timeout 1 (match (eval vm_compute in t) with
+  | xH => idtac
+  | xI ?p => assert_pos_constant p
+  | xO ?p => assert_pos_constant p
+  | _ => fail
+  end).
+
+Ltac assert_bin_constant t :=
+  timeout 1 (match (eval vm_compute in t) with
+  | N.pos ?p => assert_pos_constant p
+  | N0 => idtac
+  | _ => fail
+  end).
+
+Ltac assert_word_constant t :=
+  timeout 1 (match (eval vm_compute in t) with
+  | WO => idtac
+  | WS _ ?w => assert_word_constant w
+  | _ => fail
+  end).
+
+(** Bounding Tactics **)
+
+Ltac multi_apply0 A L := pose proof (L A).
+
+Ltac multi_apply1 A L :=
+  match goal with
+  | [ H: (wordToN A < ?b)%N |- _] => pose proof (L A b H)
+  end.
+
+Ltac multi_apply2 A B L :=
+  match goal with
+  | [ H1: (wordToN A < ?b1)%N, H2: (wordToN B < ?b2)%N |- _] => pose proof (L A B b1 b2 H1 H2)
+  end.
+
+Ltac multi_recurse n T :=
+  match goal with
+  | [ H: (wordToN T < _)%N |- _] => idtac
+  | _ =>
+    is_var T;
+    let T' := (eval cbv delta [T] in T) in multi_recurse n T';
+    match goal with
+    | [ H : T' < ?x |- _ ] =>
+      pose proof (H : T < x)
+    end
+
+  | _ =>
+    match T with
+    | ?W1 ^+ ?W2 =>
+      multi_recurse n W1; multi_recurse n W2;
+      multi_apply2 W1 W2 (@wplus_bound n)
+
+    | ?W1 ^* ?W2 =>
+      multi_recurse n W1; multi_recurse n W2;
+      multi_apply2 W1 W2 (@wmult_bound n)
+
+    | mask ?m ?w =>
+      multi_recurse n w;
+      multi_apply1 w (fun b => @mask_update_bound n w b)
+
+    | mask ?m ?w =>
+      multi_recurse n w;
+      pose proof (@mask_bound n w m)
+
+    | shiftr ?w ?bits =>
+      multi_recurse n w;
+      match goal with
+      | [ H: (w < ?b)%N |- _] =>
+        pose proof (@shiftr_bound n w b bits H)
+      end
+
+    | NToWord _ ?k => pose proof (@constant_bound_N n k)
+    | natToWord _ ?k => pose proof (@constant_bound_nat n k)
+    | _ => pose proof (@word_size_bound n T)
+    end
+  end.
+
+Lemma unwrap_let: forall {n} (y: word n) (f: word n -> word n) (b: N),
+    (&(let x := y in f x) < b)%N <-> let x := y in (&(f x) < b)%N.
+Proof. intuition. Qed.
+
+Ltac bound_compute :=
+  repeat (try assumption; match goal with
+  | [|- let A := ?B in _] =>
+    match (type of B) with
+    | word ?n => multi_recurse n B; intro
+    end
+
+  | [|- ((let A := _ in _) < _)%N] =>
+    apply unwrap_let
+
+  | [ H: (wordToN ?W < ?b0)%N |- (wordToN ?W < ?b1)%N ] =>
+    try eassumption; eapply (N.lt_le_trans _ b0 _); try eassumption
+
+  | [|- (@wordToN ?n ?W < ?b)%N ] =>
+    multi_recurse n W
+
+  | [|- (?x + ?y < ?b)%N ] =>
+    eapply plus_overflow_bound
+
+  | [|- (?a <= ?b)%N ] =>
+    is_evar b; apply N.eq_le_incl; reflexivity
+
+  | [|- (?a <= ?b)%N ] =>
+    is_evar a; apply N.eq_le_incl; reflexivity
+
+  | [|- (?a <= ?b)%N ] =>
+    assert_bin_constant a;
+    assert_bin_constant b;
+    vm_compute;
+      try reflexivity;
+      try abstract (let H := fresh in intro H; inversion H)
+
+  | [|- (?x < ?b)%N ] =>
+    assert_bin_constant x;
+    assert_bin_constant b;
+    vm_compute; reflexivity
+
+  (* cleanup generated nat goals *)
+  | [|- (?a <= ?b)%nat ] => omega
+  | [|- (?a < ?b)%nat ] => omega
+  end).
+
+(* for x : word n *)
+Ltac find_bound_on x :=
+  match (type of x) with
+  | word ?n =>
+    match x with
+    | let A := ?b in ?c => find_bound_on b; set (A := b)
+    | _ => multi_recurse n x
+    end
+  | _ => idtac
+  end.
