src/Assembly/Evaluables.v
@@ -1,0 +1,549 @@
+Require Import Bedrock.Word Bedrock.Nomega.
+Require Import NPeano NArith PArith Ndigits ZArith Znat ZArith_dec Ndec.
+Require Import List Basics Bool Nsatz Sumbool Datatypes.
+Require Import Crypto.ModularArithmetic.ModularBaseSystemOpt.
+Require Import QhasmUtil WordizeUtil Bounds.
+
+Import ListNotations.
+
+Section Evaluability.
+  Class Evaluable T := evaluator {
+    ezero: T;
+
+    (* Conversions *)
+    toT: nat -> T;
+    fromT: T -> nat;
+
+    (* Operations *)
+    eadd: T -> T -> T;
+    esub: T -> T -> T;
+    emul: T -> T -> T;
+    eshiftr: T -> nat -> T;
+    emask: T -> nat -> T;
+
+    (* Comparisons *)
+    eltb: T -> T -> bool;
+    eeqb: T -> T -> bool
+  }.
+End Evaluability.
+
+Section Z.
+  Instance ZEvaluable : Evaluable Z := {
+    ezero := 0%Z;
+
+    (* Conversions *)
+    toT := Z.of_nat;
+    fromT := Z.to_nat;
+
+    (* Operations *)
+    eadd := Z.add;
+    esub := Z.sub;
+    emul := Z.mul;
+    eshiftr := fun x k => Z.shiftr x (Z.of_nat k);
+    emask := fun x k => Z.land x (Z.ones (Z.of_nat k));
+
+    (* Comparisons *)
+    eltb := Z.ltb;
+    eeqb := Z.eqb;
+  }.
+End Z.
+
+Section Word.
+  Context {n: nat}.
+
+  Instance WordEvaluable : Evaluable (word n) := {
+    ezero := wzero n;
+
+    (* Conversions *)
+    toT := natToWord n;
+    fromT := @wordToNat n;
+
+    (* Operations *)
+    eadd := @wplus n;
+    esub := @wminus n;
+    emul := @wmult n;
+    eshiftr := @shiftr n;
+    emask := fun x k => @mask n k x;
+
+    (* Comparisons *)
+    eltb := fun x y => N.ltb (wordToN x) (wordToN y);
+    eeqb := fun x y => proj1_sig (bool_of_sumbool (@weq n x y))
+  }.
+End Word.
+
+Section RangeUpdate.
+  Context {n: nat}.
+
+  Inductive Range T := | range: forall (low high: T), Range T.
+
+  Definition validBinaryWordOp
+        (rangeF: Range N -> Range N -> option (Range N))
+        (wordF: word n -> word n -> word n): Prop :=
+    forall (low0 high0 low1 high1: N) (x y: word n),
+      (low0 <= wordToN x < high0)%N
+    -> (low1 <= wordToN y < high1)%N
+    -> match rangeF (range N low0 high0) (range N low1 high1) with
+      | Some (range low2 high2) =>
+        (low2 <= @wordToN n (wordF x y) < high2)%N
+      | _ => True 
+      end.
+
+  Definition validNatWordOp
+        (rangeF: Range N -> nat -> option (Range N))
+        (wordF: word n -> nat -> word n): Prop :=
+    forall (low0 high0: N) (k: nat) (x: word n),
+      (low0 <= wordToN x < high0)%N
+    -> match rangeF (range N low0 high0) k with
+      | Some (range low2 high2) =>
+        (low2 <= @wordToN n (wordF x k) < high2)%N
+      | _ => True 
+      end.
+
+  Section BoundedSub.
+    Lemma NToWord_Npow2: wzero n = NToWord n (Npow2 n).
+    Proof.
+      induction n as [|n0].
+
+      + repeat rewrite shatter_word_0; reflexivity.
+
+      + unfold wzero in *; simpl in *.
+        rewrite IHn0; simpl.
+        induction (Npow2 n0); simpl; reflexivity.
+    Qed.
+
+    Lemma bWSub_lem0: forall (x0 x1: word n) (low0 high1: N),
+      (low0 <= wordToN x0)%N -> (wordToN x1 < high1)%N -> 
+      (low0 - high1 <= & (x0 ^- x1))%N.
+    Proof.
+      intros.
+
+      destruct (Nge_dec (wordToN x1) 1)%N as [e|e].
+      destruct (Nge_dec (wordToN x1) (wordToN x0)).
+
+      - unfold wminus, wneg.
+        assert (low0 < high1)%N. {
+          apply (N.le_lt_trans _ (wordToN x0) _); [assumption|].
+          apply (N.le_lt_trans _ (wordToN x1) _); [apply N.ge_le|]; assumption.
+        }
+
+        replace (low0 - high1)%N with 0%N; [apply N_ge_0|].
+        symmetry.
+        apply N.sub_0_le.
+        apply N.lt_le_incl.
+        assumption.
+
+        - transitivity (wordToN x0 - wordToN x1)%N.
+
+          + transitivity (wordToN x0 - high1)%N.
+
+            * apply N.sub_le_mono_r; assumption.
+
+            * apply N.sub_le_mono_l; apply N.lt_le_incl; assumption.
+
+          + assert (& x0 - & x1 < Npow2 n)%N. {
+              transitivity (wordToN x0);
+                try apply word_size_bound;
+                apply N.sub_lt.
+
+              + apply N.lt_le_incl; assumption.
+
+              + nomega.
+            }
+
+            assert (& x0 - & x1 + & x1 < Npow2 n)%N. {
+              replace (wordToN x0 - wordToN x1 + wordToN x1)%N
+                with (wordToN x0) by nomega.
+              apply word_size_bound.
+            }
+
+            assert (x0 = NToWord n (wordToN x0 - wordToN x1) ^+ x1) as Hv. {
+              apply NToWord_equal.
+              rewrite <- wordize_plus; rewrite wordToN_NToWord;
+                try assumption.
+              nomega.
+            }
+
+            apply N.eq_le_incl.
+            rewrite Hv.
+            unfold wminus.
+            rewrite <- wplus_assoc.
+            rewrite wminus_inv.
+            rewrite (wplus_comm (NToWord n (wordToN x0 - wordToN x1)) (wzero n)).
+            rewrite wplus_unit.
+            rewrite <- wordize_plus; [nomega|].
+            rewrite wordToN_NToWord; assumption.
+
+      - unfold wminus, wneg.
+        assert (wordToN x1 = 0)%N as e' by nomega.
+        rewrite e'.
+        replace (Npow2 n - 0)%N with (Npow2 n) by nomega.
+        rewrite <- NToWord_Npow2.
+
+        erewrite <- wordize_plus;
+          try rewrite wordToN_zero;
+          replace (wordToN x0 + 0)%N with (wordToN x0)%N by nomega;
+          try apply word_size_bound.
+
+        transitivity low0; try assumption.
+        apply N.le_sub_le_add_r.
+        apply N.le_add_r.
+    Qed.
+
+    Lemma bWSub_lem1: forall (x0 x1: word n) (low1 high0: N),
+      (low1 <= wordToN x1)%N -> (wordToN x0 < high0)%N -> 
+      (& (x0 ^- x1) < N.succ (high0 + Npow2 n - low1))%N.
+    Proof.
+      intros; unfold wminus.
+      destruct (Nge_dec (wordToN x1) 1)%N as [e|e].
+      destruct (Nge_dec (wordToN x0) (wordToN x1)).
+
+      - apply N.lt_succ_r.
+        assert (& x0 - & x1 < Npow2 n)%N. {
+          transitivity (wordToN x0);
+          try apply word_size_bound;
+          apply N.sub_lt.
+
+          + apply N.ge_le; assumption.
+
+          + nomega.
+        }
+
+        assert (& x0 - & x1 + & x1 < Npow2 n)%N. {
+          replace (wordToN x0 - wordToN x1 + wordToN x1)%N
+            with (wordToN x0) by nomega.
+          apply word_size_bound.
+        }
+
+        assert (x0 = NToWord n (wordToN x0 - wordToN x1) ^+ x1) as Hv. {
+          apply NToWord_equal.
+          rewrite <- wordize_plus; rewrite wordToN_NToWord;
+          try assumption.
+          nomega.
+        }
+
+        rewrite Hv.
+        rewrite <- wplus_assoc.
+        rewrite wminus_inv.
+        rewrite wplus_comm.
+        rewrite wplus_unit.
+        rewrite wordToN_NToWord.
+
+        + transitivity (wordToN x0 - low1)%N.
+
+          * apply N.sub_le_mono_l; assumption.
+
+          * apply N.sub_le_mono_r.
+            transitivity high0; [apply N.lt_le_incl; assumption|].
+            replace' high0 with (high0 + 0)%N at 1 by nomega.
+            apply N.add_le_mono_l.
+            apply N_ge_0.
+
+        + transitivity (wordToN x0); try apply word_size_bound.
+            nomega.
+
+      - rewrite <- wordize_plus; [apply N.lt_succ_r|].
+
+        + transitivity (high0 + (wordToN (wneg x1)))%N.
+
+          * apply N.add_le_mono_r; apply N.lt_le_incl; assumption.
+
+          * unfold wneg.
+            rewrite wordToN_NToWord; [|abstract (
+              apply N.sub_lt;
+              try apply N.lt_le_incl;
+              try apply word_size_bound;
+              nomega )].
+
+            rewrite N.add_sub_assoc; [|abstract (
+              try apply N.lt_le_incl;
+              try apply word_size_bound)].
+
+            apply N.sub_le_mono_l.
+            assumption.
+
+        + unfold wneg.
+
+          rewrite wordToN_NToWord; [|abstract (
+            apply N.sub_lt;
+            try apply N.lt_le_incl;
+            try apply word_size_bound;
+            nomega )].
+
+          replace (wordToN x0 + (Npow2 n - wordToN x1))%N
+            with (Npow2 n - (wordToN x1 - wordToN x0))%N.
+
+          * apply N.sub_lt; try nomega.
+            transitivity (wordToN x1); [apply N.le_sub_l|].
+            apply N.lt_le_incl.
+            apply word_size_bound.
+
+          * apply N.add_sub_eq_l.
+            rewrite <- N.add_sub_swap;
+                [|apply N.lt_le_incl; assumption].
+            rewrite (N.add_comm (wordToN x0)).
+            rewrite N.add_assoc.
+            rewrite N.add_sub_assoc;
+                [|apply N.lt_le_incl; apply word_size_bound].
+            rewrite N.add_sub.
+            rewrite N.add_comm.
+            rewrite N.add_sub.
+            reflexivity.
+
+      - apply N.lt_succ_r.
+        assert (wordToN x1 = 0)%N as e' by nomega.
+        assert (NToWord n (wordToN x1) = NToWord n 0%N) as E by
+            (rewrite e'; reflexivity).
+        rewrite NToWord_wordToN in E.
+        simpl in E; rewrite wzero'_def in E.
+        rewrite E.
+        unfold wneg.
+        rewrite wordToN_zero.
+        rewrite N.sub_0_r.
+        rewrite <- NToWord_Npow2.
+        rewrite wplus_comm.
+        rewrite wplus_unit.
+        transitivity high0.
+
+        + apply N.lt_le_incl.
+          assumption.
+
+        + rewrite <- N.add_sub_assoc.
+
+          * replace high0 with (high0 + 0)%N by nomega.
+            apply N.add_le_mono; [|apply N_ge_0].
+            apply N.eq_le_incl.
+            rewrite N.add_0_r.
+            reflexivity.
+
+          * transitivity (wordToN x1);
+            [ assumption
+            | apply N.lt_le_incl;
+                apply word_size_bound].
+
+    Qed.
+  End BoundedSub.
+
+  Lemma range_add_valid :
+    validBinaryWordOp
+      (fun range0 range1 =>
+         match (range0, range1) with
+         | (range low0 high0, range low1 high1) =>
+           if (overflows n (high0 + high1))
+           then None
+           else Some (range N (low0 + low1) (high0 + high1))
+         end)%N
+      (@wplus n).
+  Proof.
+    unfold validBinaryWordOp; intros until y; intros H0 H1.
+    destruct H0 as [H0a H0b].
+    destruct H1 as [H1a H1b].
+
+    destruct (overflows n (high0 + high1))%N; split.
+
+    - erewrite <- wordize_plus';
+        try eassumption;
+        try abstract nomega.
+
+      + apply N.add_le_mono; assumption.
+
+      + apply N.lt_le_incl; nomega.
+
+    - apply (N.le_lt_trans _ (wordToN x + wordToN y)%N _);
+        try apply plus_le.
+      nomega.
+  Qed.
+
+  Lemma range_sub_valid :
+    validBinaryWordOp
+      (fun range0 range1 =>
+         match (range0, range1) with
+         | (range low0 high0, range low1 high1) =>
+           if (Nge_dec low0 high1)
+           then Some (range N (low0 - high1)%N
+              (if (Nge_dec high0 (Npow2 n)) then Npow2 n else
+               if (Nge_dec high1 (Npow2 n)) then Npow2 n else
+               N.succ (high0 + Npow2 n - low1))%N)
+           else None
+         end)
+      (@wminus n).
+  Proof.
+    unfold validBinaryWordOp; intros until y; intros H0 H1.
+    destruct H0 as [H0a H0b].
+    destruct H1 as [H1a H1b].
+
+    destruct (Nge_dec high0 (Npow2 n)),
+             (Nge_dec high1 (Npow2 n)),
+             (Nge_dec low0 high1); split;
+      repeat match goal with
+      | [|- (_ - ?x <= wordToN _)%N] => apply bWSub_lem0
+      | [|- (wordToN _ < N.succ (?x + _ - _))%N] => apply bWSub_lem1
+      | [|- (wordToN _ < Npow2 _)%N] => apply word_size_bound
+      | [|- (0 <= _)%N] => apply N_ge_0
+      end; assumption.
+  Qed.
+
+  Lemma range_mul_valid :
+    validBinaryWordOp
+      (fun range0 range1 =>
+         match (range0, range1) with
+         | (range low0 high0, range low1 high1) =>
+           if (overflows n (high0 * high1)) then None else
+           Some (range N (low0 * low1) (high0 * high1))%N
+          end)
+      (@wmult n).
+  Proof.
+    unfold validBinaryWordOp; intros until y; intros H0 H1.
+    destruct H0 as [H0a H0b].
+    destruct H1 as [H1a H1b].
+
+    destruct (overflows n (high0 * high1))%N; split.
+
+    - rewrite <- wordize_mult.
+
+      + apply N.mul_le_mono; assumption.
+
+      + transitivity (high0 * high1)%N; [|assumption].
+        apply N.mul_lt_mono; assumption.
+
+    - apply (N.le_lt_trans _ (wordToN x * wordToN y)%N _); [apply mult_le|].
+      apply N.mul_lt_mono; assumption.
+  Qed.
+
+  Lemma range_shiftr_valid :
+    validNatWordOp
+      (fun range0 k =>
+         match range0 with
+         | range low high =>
+           Some (range N
+             (N.shiftr low (N.of_nat k))
+             (N.succ (N.shiftr high (N.of_nat k))))
+          end)
+      (fun x k => extend (Nat.eq_le_incl _ _ eq_refl) (shiftr x k)).
+  Proof.
+    unfold validNatWordOp; intros until x; intro H.
+    destruct H as [Ha Hb]; split.
+
+    - unfold extend; rewrite wordToN_convS.
+
+      rewrite wordToN_zext.
+      rewrite <- wordize_shiftr.
+      rewrite <- Nshiftr_equiv_nat.
+      repeat rewrite N.shiftr_div_pow2.
+      apply N.div_le_mono; [|assumption].
+      induction k.
+
+      + cbv beta delta iota; intro Z; inversion Z.
+
+      + rewrite <- Npow2_N.
+        pose proof (Npow2_gt0 (S k)).
+        nomega.
+
+    - unfold extend; rewrite wordToN_convS.
+      rewrite wordToN_zext.
+      rewrite Nshiftr_equiv_nat.
+      eapply N.lt_le_trans.
+
+      + apply shiftr_bound; eassumption.
+
+      + apply N.eq_le_incl.
+        reflexivity.
+  Qed.
+
+  Lemma range_mask_valid :
+    validNatWordOp
+      (fun range0 k =>
+         match range0 with
+         | range low high =>
+           Some (range N 0%N (Npow2 k))
+          end)
+      (fun x k => mask k x).
+  Proof.
+    unfold validNatWordOp; intros until x; intro H.
+    destruct H as [Ha Hb]; split; [apply N_ge_0|].
+    apply mask_bound.
+  Qed.
+End RangeUpdate.
+
+Section WordRange.
+  Context {n: nat}.
+
+  Inductive WordRangeOpt :=
+    | someRange: forall (low high: N),
+        (low < high)%N -> (high <= Npow2 n)%N -> WordRangeOpt
+    | applyBinOp: forall rangeF wordF,
+        @validBinaryWordOp n rangeF wordF ->
+        WordRangeOpt -> WordRangeOpt -> WordRangeOpt
+    | applyNatOp: forall rangeF wordF,
+        @validNatWordOp n rangeF wordF ->
+        WordRangeOpt -> nat -> WordRangeOpt.
+
+  Fixpoint evalWordRangeOpt (r: WordRangeOpt): option (Range N) :=
+    match r with
+    | someRange low high _ _ => Some (range N low high)
+    | applyBinOp rangeF wordF _ a b =>
+      omap (evalWordRangeOpt a) (fun a' =>
+        omap (evalWordRangeOpt a) (fun b' =>
+          rangeF a' b'))
+    | applyNatOp rangeF wordF _ x k =>
+      omap (evalWordRangeOpt x) (fun x' =>
+        rangeF x' k)
+    end.
+
+  Definition anyWord: WordRangeOpt.
+    refine (someRange 0%N (Npow2 n) _ _).
+    - apply Npow2_gt0.
+    - reflexivity.
+  Defined.
+
+  Definition getLowerBoundOpt (w: WordRangeOpt): option N :=
+    omap (evalWordRangeOpt w) (fun r =>
+      match r with | range low high => Some low end).
+
+  Definition getUpperBoundOpt (w: WordRangeOpt): option N :=
+    omap (evalWordRangeOpt w) (fun r =>
+      match r with | range low high => Some high end).
+
+  Definition makeRangeOpt (low high: N): option WordRangeOpt.
+    refine (
+      match (Nge_dec low high, Nge_dec high (Npow2 n)) with
+      | (right _, right _) => Some (someRange low high _ _)
+      | _ => None
+      end); [assumption|].
+
+    apply N.lt_le_incl; assumption.
+  Defined.
+
+  Definition getOrElse {T} (d: T) (o: option T) :=
+    match o with | Some x => x | None => d end.
+
+  Instance WordRangeOptEvaluable : Evaluable WordRangeOpt := {
+    ezero := anyWord;
+
+    (* Conversions *)
+    toT := fun x => getOrElse anyWord (makeRangeOpt 0%N (N.of_nat x));
+    fromT := fun x => getOrElse (pow2 n) (option_map N.to_nat (getUpperBoundOpt x));
+
+    (* Operations *)
+    eadd := applyBinOp _ _ range_add_valid;
+    esub := applyBinOp _ _ range_sub_valid;
+    emul := applyBinOp _ _ range_mul_valid;
+    eshiftr := applyNatOp _ _ range_shiftr_valid;
+    emask := applyNatOp _ _ range_mask_valid;
+
+    (* Comparisons just test upper bounds.
+       We won't bounds-check Ite in our PHOAS formalism *)
+    eltb := fun x y =>
+      getOrElse false (
+        omap (getUpperBoundOpt x) (fun xb =>
+          omap (getUpperBoundOpt y) (fun yb =>
+            Some (N.ltb xb yb))));
+
+    eeqb := fun x y =>
+      getOrElse false (
+        omap (getUpperBoundOpt x) (fun xub =>
+          omap (getUpperBoundOpt y) (fun yub =>
+            omap (getLowerBoundOpt x) (fun xlb =>
+              omap (getLowerBoundOpt y) (fun ylb =>
+                Some (andb (N.eqb xub yub) (N.eqb xlb ylb)))))))
+  }.
+End WordRange.
