src/Assembly/Listize.v
@@ -1,0 +1,108 @@
+Require Export Bedrock.Word Bedrock.Nomega.
+Require Import NPeano NArith PArith Ndigits Compare_dec Arith.
+Require Import ProofIrrelevance Ring List Omega.
+Require Import Program.Equality.
+Require Import Crypto.Util.Tuple.
+
+Definition Let_In {A P} (x : A) (f : forall a : A, P a) : P x :=
+  let y := x in f y.
+
+Notation "'plet' x := y 'in' z" := (Let_In y (fun x => z)) (at level 60).
+
+Section Listize.
+  Import ListNotations.
+
+  Transparent tuple.
+
+  Fixpoint tupleToList' {A k}: tuple' A k -> list A :=
+    match k as k' return tuple' A k' -> list A with
+    | O => fun x => [x]
+    | (S k'') => fun x =>
+      match x with
+      | (t, v) => v :: (@tupleToList' _ _ t)
+      end
+    end.
+
+  Definition tupleToList {A} (k: nat): tuple A k -> list A :=
+    match k as k' return tuple A k' -> list A with
+    | O => fun _ => []
+    | (S k'') => @tupleToList' A k''
+    end.
+
+  Lemma app_cons: forall {T} (x: T) (lst: list T), [x] ++ lst = cons x lst.
+  Proof. intros; simpl; reflexivity. Qed.
+
+  Fixpoint Curried (A B: Type) (ins: nat) (outs: nat): Type :=
+    match ins with
+    | O => list B
+    | S ins' => A -> (Curried A B ins' outs)
+    end.
+
+  Definition ListF (A B: Type): Type := list A -> list B.
+
+  Fixpoint curriedToListF' {A B: Type} {ins outs: nat} (args: nat) (default: A)
+      (f: Curried A B ins outs): ListF A B := fun (lst: list A) =>
+    match ins as ins' return Curried A B ins' outs -> list B with
+    | O => fun g => g
+    | S ins'' => fun g =>
+      (curriedToListF' args default (g (nth (args - ins) lst default))) lst
+    end f.
+
+  Definition curriedToListF {A B: Type} {ins outs: nat} (default: A)
+      (f: Curried A B ins outs): ListF A B :=
+    curriedToListF' ins default f.
+
+End Listize.
+
+Section Lets.
+  Import ListNotations.
+
+  Lemma detuple_let: forall {A B C} (y0: A) (y1: B) (z: (A * B) -> C),
+      Let_In (y0, y1) z =
+        Let_In y0 (fun x0 =>
+          Let_In y1 (fun x1 =>
+            z (x0, x1))).
+  Proof. intros; unfold Let_In; cbv zeta; intuition. Qed.
+
+  Lemma listize_let: forall {A B} (y d: A) (z: A -> B),
+      Let_In y z = Let_In [y] (fun x => z (nth 0 x d)).
+  Proof. intros; unfold Let_In; cbv zeta; intuition. Qed.
+
+  Lemma combine_let_lists: forall {A B} (a: list A) (b: list A) (d: A) (z: list A -> list A -> B),
+      Let_In a (fun x => Let_In b (z x)) =
+        Let_In (a ++ b) (fun x => z (firstn (length a) x) (skipn (length a) x)).
+  Proof.
+
+    intros; unfold Let_In; cbv zeta.
+
+    assert (forall b0, firstn (length a) (a ++ b0) = a) as HA. {
+      induction a; intros; simpl; try reflexivity.
+      apply f_equal; apply IHa.
+    }
+
+    assert (forall b0, skipn (length a) (a ++ b0) = b0) as HB. {
+      induction a; intros; simpl; try reflexivity.
+      apply IHa; intro; simpl in HA.
+      pose proof (HA b1) as HA'; inversion HA' as [HA''].
+      rewrite HA''.
+      assumption.
+    }
+
+    rewrite HA, HB; reflexivity.
+  Qed.
+
+End Lets.
+
+Ltac list_destruct :=
+  repeat match goal with
+  | [H: context[Datatypes.length (cons _ _)] |- _] => simpl in H
+  | [H: context[Datatypes.length nil] |- _] => simpl in H
+  | [H: S ?a = S ?b |- _] => inversion H; clear H
+  | [H: (S ?a) = 0 |- _] => contradict H; intuition
+  | [H: 0 = (S ?a) |- _] => contradict H; intuition
+  | [H: 0 = 0 |- _] => clear H
+  | [x: list ?T |- _] =>
+    match goal with
+    | [H: context[Datatypes.length x] |- _] => destruct x
+    end
+  end.
