src/Assembly/WordizeUtil.v
@@ -1,0 +1,905 @@
+Require Import Bedrock.Word Bedrock.Nomega.
+Require Import NArith PArith Ndigits Nnat NPow NPeano Ndec.
+Require Import List Omega NArith Nnat BoolEq Compare_dec.
+Require Import SetoidTactics.
+Require Import ProofIrrelevance FunctionalExtensionality.
+Require Import QhasmUtil QhasmEvalCommon.
+
+(* Custom replace-at wrapper for 8.4pl3 compatibility *)
+Definition ltac_nat_from_int (x:BinInt.Z) : nat :=
+  match x with
+  | BinInt.Z0 => 0%nat
+  | BinInt.Zpos p => BinPos.nat_of_P p
+  | BinInt.Zneg p => 0%nat
+  end.
+
+Ltac nat_from_number N :=
+  match type of N with
+  | nat => constr:(N)
+  | BinInt.Z => let N' := constr:(ltac_nat_from_int N) in eval compute in N'
+  end.
+
+Tactic Notation "replace'" constr(x) "with" constr(y) "at" constr(n) "by" tactic(tac) :=
+  let tmp := fresh in (
+  match nat_from_number n with
+  | 1 => set (tmp := x) at 1
+  | 2 => set (tmp := x) at 2
+  | 3 => set (tmp := x) at 3
+  | 4 => set (tmp := x) at 4
+  | 5 => set (tmp := x) at 5
+  end;
+    replace tmp with y by (unfold tmp; tac);
+    clear tmp).
+
+(* Word-shattering tactic *)
+Ltac shatter a :=
+  let H := fresh in
+  pose proof (shatter_word a) as H; simpl in H;
+    try rewrite H in *; clear H.
+
+Section Misc.
+  Local Open Scope nword_scope.
+
+  Lemma word_replace: forall n m, n = m -> word n = word m.
+  Proof. intros; subst; intuition. Qed.
+
+  Lemma of_nat_lt: forall x b, (x < b)%nat <-> (N.of_nat x < N.of_nat b)%N.
+  Proof.
+    intros x b; split; intro H.
+
+    - unfold N.lt; rewrite N2Nat.inj_compare.
+      repeat rewrite Nat2N.id.
+      apply nat_compare_lt in H.
+      intuition.
+
+    - unfold N.lt in H; rewrite N2Nat.inj_compare in H.
+      repeat rewrite Nat2N.id in H.
+      apply nat_compare_lt in H.
+      intuition.
+  Qed.
+
+  Lemma to_nat_lt: forall x b, (x < b)%N <-> (N.to_nat x < N.to_nat b)%nat.
+  Proof.
+    intros x b; split; intro H.
+
+    - unfold N.lt in H; rewrite N2Nat.inj_compare in H.
+      apply nat_compare_lt in H.
+      intuition.
+
+    - unfold N.lt; rewrite N2Nat.inj_compare.
+      apply nat_compare_lt.
+      intuition.
+  Qed.
+
+  Lemma word_size_bound : forall {n} (w: word n), (&w < Npow2 n)%N.
+  Proof.
+    intros; pose proof (wordToNat_bound w) as B;
+      rewrite of_nat_lt in B;
+      rewrite <- Npow2_nat in B;
+      rewrite N2Nat.id in B;
+      rewrite <- wordToN_nat in B;
+      assumption.
+  Qed.
+
+  Lemma ge_to_le: forall (x y: N), (x >= y)%N <-> (y <= x)%N.
+  Proof.
+    intros x y; split; intro H;
+      unfold N.ge, N.le in *;
+      intro H0; contradict H;
+      rewrite N.compare_antisym;
+      rewrite H0; simpl; intuition.
+  Qed.
+
+  Lemma N_ge_0: forall x: N, (0 <= x)%N.
+  Proof.
+    intro x0; unfold N.le.
+    pose proof (N.compare_0_r x0) as H.
+    rewrite N.compare_antisym in H.
+    induction x0; simpl in *;
+      intro V; inversion V.
+  Qed.
+
+  Lemma Pos_ge_1: forall p, (1 <= N.pos p)%N.
+  Proof.
+    intro.
+    replace (N.pos p) with (N.succ (N.pos p - 1)%N) by (
+      induction p; simpl;
+      try rewrite Pos.succ_pred_double;
+      try reflexivity).
+    unfold N.succ.
+    apply N.le_pred_le_succ.
+    replace (N.pred 1%N) with 0%N by (simpl; intuition).
+    apply N_ge_0.
+  Qed.
+
+  Lemma testbit_wones_false: forall n k,
+     (k >= N.of_nat n)%N
+   -> false = N.testbit (& wones n) k.
+  Proof.
+    induction n; try abstract (simpl; intuition).
+    induction k; try abstract (
+      intro H; destruct H; simpl; intuition).
+
+    intro H.
+    assert (N.pos p - 1 >= N.of_nat n)%N as Z.
+      apply ge_to_le;
+      apply ge_to_le in H;
+      apply (N.add_le_mono_r _ _ 1%N);
+      replace (N.of_nat n + 1)%N with (N.of_nat (S n));
+      replace (N.pos p - 1 + 1)%N with (N.pos p);
+      try rewrite N.sub_add;
+      try assumption;
+      try nomega;
+      apply Pos_ge_1.
+
+    rewrite (IHn (N.pos p - 1)%N Z) at 1.
+
+    assert (N.pos p = N.succ (N.pos p - 1)) as Hp by (
+      rewrite <- N.pred_sub;
+      rewrite N.succ_pred;
+      try abstract intuition;
+      intro H0; inversion H0).
+
+    symmetry.
+    rewrite Hp at 1.
+    rewrite Hp in H.
+
+    revert H; clear IHn Hp Z;
+      generalize (N.pos p - 1)%N as x;
+      intros x H.
+
+    replace (& wones (S n)) with (2 * & (wones n) + N.b2n true)%N
+      by (simpl; nomega).
+
+    rewrite N.testbit_succ_r; reflexivity.
+  Qed.
+
+  Lemma testbit_wones_true: forall n k,
+     (k < N.of_nat n)%N
+   -> true = N.testbit (& wones n) k.
+  Proof.
+    induction n; intros k H; try nomega.
+    destruct (N.eq_dec k (N.of_nat n)).
+
+    - clear IHn H; subst.
+      induction n.
+
+      + simpl; intuition.
+
+      + replace (& (wones (S (S n))))
+           with (2 * (& (wones (S n))) + N.b2n true)%N
+          by (simpl; nomega).
+        rewrite Nat2N.inj_succ.
+        rewrite N.testbit_succ_r.
+        assumption.
+
+    - induction k.
+
+      + replace (& (wones (S n))) with (2 * (& (wones n)) + N.b2n true)%N
+          by (simpl; nomega).
+        rewrite N.testbit_0_r.
+        reflexivity.
+
+      + assert (N.pos p < N.of_nat n)%N as IH by (
+          rewrite Nat2N.inj_succ in H;
+          nomega).
+        apply N.lt_lt_pred in IH.
+        apply IHn in IH.
+        replace (N.pos p) with (N.succ (N.pred (N.pos p))) by (
+          induction p; simpl;
+          try rewrite Pos.succ_pred_double;
+          intuition).
+        replace (& (wones (S n))) with (2 * (& (wones n)) + N.b2n true)%N
+          by (simpl; nomega).
+        rewrite N.testbit_succ_r.
+        assumption.
+  Qed.
+
+  
+  Lemma plus_le: forall {n} (x y: word n),
+    (& (x ^+ y) <= &x + &y)%N.
+  Proof.
+    intros.
+    unfold wplus, wordBin.
+    rewrite wordToN_nat.
+    rewrite NToWord_nat.
+    pose proof (wordToNat_natToWord n (N.to_nat (& x + & y))) as H.
+    destruct H as [k H].
+    destruct H as [Heq Hk].
+    rewrite Heq.
+    rewrite Nat2N.inj_sub.
+    rewrite N2Nat.id.
+    generalize (&x + &y)%N; intro a.
+    generalize (N.of_nat (k * pow2 n))%N; intro b.
+    clear Heq Hk; clear x y k; clear n.
+    replace a with (a - 0)%N by nomega.
+    replace' (a - 0)%N with a at 1 by nomega.
+    apply N.sub_le_mono_l.
+    apply N_ge_0.
+  Qed.
+
+  Lemma mult_le: forall {n} (x y: word n),
+    (& (x ^* y) <= &x * &y)%N.
+  Proof.
+    intros.
+    unfold wmult, wordBin.
+    rewrite wordToN_nat.
+    rewrite NToWord_nat.
+    pose proof (wordToNat_natToWord n (N.to_nat (& x * & y))) as H.
+    destruct H as [k H].
+    destruct H as [Heq Hk].
+    rewrite Heq.
+    rewrite Nat2N.inj_sub.
+    rewrite N2Nat.id.
+    generalize (&x * &y)%N; intro a.
+    generalize (N.of_nat (k * pow2 n))%N; intro b.
+    clear Heq Hk; clear x y k; clear n.
+    replace a with (a - 0)%N by nomega.
+    replace' (a - 0)%N with a at 1 by nomega.
+    apply N.sub_le_mono_l.
+    apply N_ge_0.
+  Qed.
+End Misc.
+
+Section Exp.
+  Local Open Scope nword_scope.
+
+  Lemma pow2_inv : forall n m, pow2 n = pow2 m -> n = m.
+  Proof.
+    induction n; intros; simpl in *;
+        induction m; simpl in *; try omega.
+    f_equal; apply IHn.
+    omega.
+  Qed.
+
+  Lemma pow2_gt0 : forall n, (pow2 n > O)%nat.
+  Proof. induction n; simpl; omega. Qed.
+
+  Lemma pow2_N_bound: forall n j,
+    (j < pow2 n)%nat -> (N.of_nat j < Npow2 n)%N.
+  Proof.
+    intros.
+    rewrite <- Npow2_nat in H.
+    unfold N.lt.
+    rewrite N2Nat.inj_compare.
+    rewrite Nat2N.id.
+    apply nat_compare_lt in H.
+    assumption.
+  Qed.
+
+  Lemma Npow2_gt0 : forall x, (0 < Npow2 x)%N.
+  Proof.
+    intros; induction x.
+
+    - simpl; apply N.lt_1_r; intuition.
+
+    - replace (Npow2 (S x)) with (2 * (Npow2 x))%N by intuition.
+        apply (N.lt_0_mul 2 (Npow2 x)); left; split; apply N.neq_0_lt_0.
+
+      + intuition; inversion H.
+
+      + apply N.neq_0_lt_0 in IHx; intuition.
+  Qed.
+
+  Lemma Npow2_ge1 : forall x, (1 <= Npow2 x)%N.
+  Proof.
+    intro x.
+    pose proof (Npow2_gt0 x) as Z.
+    apply N.lt_pred_le; simpl.
+    assumption.
+  Qed.
+
+  Lemma Npow2_split: forall a b,
+    (Npow2 (a + b) = (Npow2 a) * (Npow2 b))%N.
+  Proof.
+    intros; revert a.
+    induction b.
+
+    - intros; simpl; replace (a + 0) with a; try nomega.
+      rewrite N.mul_1_r; intuition.
+
+    - intros.
+      replace (a + S b) with (S a + b) by omega.
+      rewrite (IHb (S a)); simpl; clear IHb.
+      induction (Npow2 a), (Npow2 b); simpl; intuition.
+      rewrite Pos.mul_xO_r; intuition.
+  Qed.
+
+  Lemma Npow2_N: forall n, Npow2 n = (2 ^ N.of_nat n)%N.
+  Proof.
+    induction n.
+
+    - simpl; intuition.
+
+    - rewrite Nat2N.inj_succ.
+      rewrite N.pow_succ_r; try apply N_ge_0.
+      rewrite <- IHn.
+      simpl; intuition.
+  Qed.
+ 
+  Lemma Npow2_succ: forall n, (Npow2 (S n) = 2 * (Npow2 n))%N.
+  Proof. intros; simpl; induction (Npow2 n); intuition. Qed.
+
+  Lemma Npow2_ordered: forall n m, (n <= m)%nat -> (Npow2 n <= Npow2 m)%N.
+  Proof.
+    induction n; intros m H; try rewrite Npow2_succ.
+
+    - simpl; apply Npow2_ge1.
+
+    - induction m; try rewrite Npow2_succ.
+
+      + inversion H.
+
+      + assert (n <= m)%nat as H0 by omega.
+        apply IHn in H0.
+        apply N.mul_le_mono_l.
+        assumption.
+  Qed.
+
+End Exp.
+
+Section Conversions.
+  Local Open Scope nword_scope.
+
+  Lemma NToWord_wordToN: forall sz x, NToWord sz (wordToN x) = x.
+  Proof.
+    intros.
+    rewrite NToWord_nat.
+    rewrite wordToN_nat.
+    rewrite Nat2N.id.
+    rewrite natToWord_wordToNat.
+    intuition.
+  Qed.
+
+  Lemma NToWord_equal: forall n (x y: word n),
+      wordToN x = wordToN y -> x = y.
+  Proof.
+    intros.
+    rewrite <- (NToWord_wordToN _ x).
+    rewrite <- (NToWord_wordToN _ y).
+    rewrite H; reflexivity.
+  Qed.
+
+  Lemma wordToN_NToWord: forall sz x, (x < Npow2 sz)%N -> wordToN (NToWord sz x) = x.
+  Proof.
+    intros.
+    rewrite NToWord_nat.
+    rewrite wordToN_nat.
+    rewrite <- (N2Nat.id x).
+    apply Nat2N.inj_iff.
+    rewrite Nat2N.id.
+    apply natToWord_inj with (sz:=sz);
+      try rewrite natToWord_wordToNat;
+      intuition.
+
+    - apply wordToNat_bound.
+    - rewrite <- Npow2_nat; apply to_nat_lt; assumption.
+  Qed.
+
+  Lemma Npow2_ignore: forall {n} (x: word n),
+    x = NToWord _ (& x + Npow2 n).
+  Proof.
+    intros.
+    rewrite <- (NToWord_wordToN n x) at 1.
+    repeat rewrite NToWord_nat.
+    rewrite N2Nat.inj_add.
+    rewrite Npow2_nat.
+    replace' (N.to_nat (&x))
+       with ((N.to_nat (&x) + pow2 n) - 1 * pow2 n)
+         at 1 by omega.
+    rewrite drop_sub; [intuition|omega].
+  Qed.
+End Conversions.
+
+Section SpecialFunctions.
+  Local Open Scope nword_scope.
+
+  Lemma convS_id: forall n x p, (@convS n n x p) = x.
+  Proof.
+    intros; unfold convS; vm_compute.
+    replace (convS_subproof n n x p)
+      with (eq_refl (word n)) by (apply proof_irrelevance).
+    reflexivity.
+  Qed.
+
+  Lemma wordToN_convS: forall {n m} x p,
+    wordToN (@convS n m x p) = wordToN x.
+  Proof.
+    intros.
+    revert x.
+    rewrite p.
+    intro x.
+    rewrite convS_id.
+    reflexivity.
+  Qed.
+
+  Lemma wordToN_zext: forall {n m} (x: word n),
+    wordToN (@zext n x m) = wordToN x.
+  Proof.
+    intros; induction x; simpl; intuition.
+
+    - unfold zext, Word.combine.
+      rewrite wordToN_nat.
+      unfold wzero.
+      rewrite (@wordToNat_natToWord_idempotent m 0); simpl; intuition.
+      apply Npow2_gt0.
+
+    - unfold zext in IHx; rewrite IHx; clear IHx;
+        destruct b; intuition.
+  Qed.
+
+  Lemma wordToN_div2: forall {n} (x: word (S n)),
+    N.div2 (&x) = & (wtl x).
+  Proof.
+    intros.
+    pose proof (shatter_word x) as Hx; simpl in Hx; rewrite Hx; simpl.
+    destruct (whd x).
+    replace (match & wtl x with
+             | 0%N => 0%N
+             | N.pos q => N.pos (xO q)
+             end)
+       with (N.double (& (wtl x)))
+         by (induction (& (wtl x)); simpl; intuition).
+
+    - rewrite N.double_spec.
+      replace (N.succ (2 * & wtl x))
+         with ((2 * (& wtl x)) + 1)%N
+           by nomega.
+      rewrite <- N.succ_double_spec.
+      rewrite N.div2_succ_double.
+      reflexivity.
+
+    - induction (& (wtl x)); simpl; intuition.
+  Qed.
+
+  Fixpoint wbit {n} (x: word n) (k: nat): bool :=
+    match n as n' return word n' -> bool with
+    | O => fun _ => false
+    | S m => fun x' =>
+      match k with
+      | O => (whd x')
+      | S k' => wbit (wtl x') k'
+      end
+    end x.
+
+  Lemma wbit_wtl: forall {n} (x: word (S n)) k,
+    wbit x (S k) = wbit (wtl x) k.
+  Proof.
+    intros.
+    pose proof (shatter_word x) as Hx;
+      simpl in Hx; rewrite Hx; simpl.
+    reflexivity.
+  Qed.
+
+  Lemma wordToN_testbit: forall {n} (x: word n) k,
+    N.testbit (& x) k = wbit x (N.to_nat k).
+  Proof.
+    assert (forall x: N, match x with
+            | 0%N => 0%N
+            | N.pos q => N.pos (q~0)%positive
+            end = N.double x) as kill_match by (
+      induction x; simpl; intuition).
+
+    induction n; intros.
+
+    - shatter x; simpl; intuition.
+
+    - revert IHn; rewrite <- (N2Nat.id k).
+      generalize (N.to_nat k) as k'; intros; clear k.
+      rewrite Nat2N.id in *.
+
+      induction k'.
+
+      + clear IHn; induction x; simpl; intuition.
+        destruct (& x), b; simpl; intuition. 
+
+      + clear IHk'.
+        shatter x; simpl.
+
+        rewrite kill_match.
+        replace (N.pos (Pos.of_succ_nat k'))
+           with (N.succ (N.of_nat k'))
+             by (rewrite <- Nat2N.inj_succ;
+                 simpl; intuition).
+
+        rewrite N.double_spec.
+        replace (N.succ (2 * & wtl x))
+           with (2 * & wtl x + 1)%N
+             by nomega.
+
+        destruct (whd x);
+          try rewrite N.testbit_odd_succ;
+          try rewrite N.testbit_even_succ;
+          try abstract (
+            unfold N.le; simpl;
+            induction (N.of_nat k'); intuition;
+            try inversion H);
+          rewrite IHn;
+          rewrite Nat2N.id;
+          reflexivity.
+  Qed.
+ 
+  Lemma wordToN_split1: forall {n m} x,
+    & (@split1 n m x) = N.land (& x) (& (wones n)).
+  Proof.
+    intros.
+
+    pose proof (Word.combine_split _ _ x) as C; revert C.
+    generalize (split1 n m x) as a, (split2 n m x) as b.
+    intros a b C; rewrite <- C; clear C x.
+
+    apply N.bits_inj_iff; unfold N.eqf; intro x.
+    rewrite N.land_spec.
+    repeat rewrite wordToN_testbit.
+    revert x a b.
+
+    induction n, m; intros;
+      shatter a; shatter b;
+      induction (N.to_nat x) as [|n0];
+      try rewrite <- (Nat2N.id n0);
+      try rewrite andb_false_r;
+      try rewrite andb_true_r;
+      simpl; intuition.
+  Qed.
+
+  Lemma wordToN_split2: forall {n m} x,
+    & (@split2 n m x) = N.shiftr (& x) (N.of_nat n).
+  Proof.
+    intros.
+
+    pose proof (Word.combine_split _ _ x) as C; revert C.
+    generalize (split1 n m x) as a, (split2 n m x) as b.
+    intros a b C.
+    rewrite <- C; clear C x.
+
+    apply N.bits_inj_iff; unfold N.eqf; intro x;
+      rewrite N.shiftr_spec;
+      repeat rewrite wordToN_testbit;
+      try apply N_ge_0.
+
+    revert x a b.
+    induction n, m; intros;
+      shatter a;
+      try apply N_ge_0.
+
+    - simpl; intuition.
+
+    - replace (x + N.of_nat 0)%N with x by nomega.
+      simpl; intuition.
+
+    - rewrite (IHn x (wtl a) b).
+      rewrite <- (N2Nat.id x).
+      repeat rewrite <- Nat2N.inj_add.
+      repeat rewrite Nat2N.id; simpl.
+      replace (N.to_nat x + S n) with (S (N.to_nat x + n)) by omega.
+      reflexivity.
+
+    - rewrite (IHn x (wtl a) b).
+      rewrite <- (N2Nat.id x).
+      repeat rewrite <- Nat2N.inj_add.
+      repeat rewrite Nat2N.id; simpl.
+      replace (N.to_nat x + S n) with (S (N.to_nat x + n)) by omega.
+      reflexivity.
+  Qed.
+
+  Lemma wordToN_combine: forall {n m} a b,
+    & (@Word.combine n a m b) = N.lxor (N.shiftl (& b) (N.of_nat n)) (& a).
+  Proof.
+    intros; symmetry.
+
+    replace' a with (Word.split1 _ _ (Word.combine a b)) at 1
+      by (apply Word.split1_combine).
+
+    replace' b with (Word.split2 _ _ (Word.combine a b)) at 1
+      by (apply Word.split2_combine).
+
+    generalize (Word.combine a b); intro x; clear a b.
+
+    rewrite wordToN_split1, wordToN_split2.
+    generalize (&x); clear x; intro x.
+    apply N.bits_inj_iff; unfold N.eqf; intro k.
+
+    rewrite N.lxor_spec.
+    destruct (Nge_dec k (N.of_nat n)).
+
+    - rewrite N.shiftl_spec_high; try apply N_ge_0;
+        try (apply ge_to_le; assumption).
+      rewrite N.shiftr_spec; try apply N_ge_0.
+      replace (k - N.of_nat n + N.of_nat n)%N with k by nomega.
+      rewrite N.land_spec.
+      induction (N.testbit x k); 
+        replace (N.testbit (& wones n) k) with false;
+        simpl; intuition;
+        try apply testbit_wones_false;
+        try assumption.
+
+    - rewrite N.shiftl_spec_low; try assumption; try apply N_ge_0.
+      rewrite N.land_spec.
+      induction (N.testbit x k);
+        replace (N.testbit (& wones n) k) with true;
+        simpl; intuition;
+        try apply testbit_wones_true;
+        try assumption.
+  Qed.
+
+  Lemma wordToN_wones: forall x, & (wones x) = N.ones (N.of_nat x).
+  Proof.
+    induction x.
+
+    - simpl; intuition.
+
+    - rewrite Nat2N.inj_succ.
+      replace (& wones (S x)) with (2 * & (wones x) + N.b2n true)%N
+        by (simpl; nomega).
+      replace (N.ones (N.succ _))
+         with (2 * N.ones (N.of_nat x) + N.b2n true)%N.
+
+      + rewrite IHx; nomega.
+
+      + replace (N.succ (N.of_nat x)) with (1 + (N.of_nat x))%N by (
+          rewrite N.add_comm; nomega).
+        rewrite N.ones_add.
+        replace (N.ones 1) with 1%N by (
+          unfold N.ones; simpl; intuition).
+        simpl.
+        reflexivity.
+  Qed.
+
+  Lemma wordToN_zero: forall w, wordToN (wzero w) = 0%N.
+  Proof.
+    intros.
+    unfold wzero; rewrite wordToN_nat.
+    rewrite wordToNat_natToWord_idempotent; simpl; intuition.
+    apply Npow2_gt0.
+  Qed.
+
+  Lemma NToWord_zero: forall w, NToWord w 0%N = wzero w.
+  Proof.
+    intros.
+    unfold wzero; rewrite NToWord_nat.
+    f_equal.
+  Qed.
+
+  Ltac propagate_wordToN :=
+    unfold extend, low, high, break;
+    repeat match goal with
+    | [|- context[@wordToN _ (@convS _ _ _ _)] ] =>
+      rewrite wordToN_convS
+    | [|- context[@wordToN _ (@split1 _ _ _)] ] =>
+      rewrite wordToN_split1
+    | [|- context[@wordToN _ (@split2 _ _ _)] ] =>
+      rewrite wordToN_split2
+    | [|- context[@wordToN _ (@combine _ _ _ _)] ] =>
+      rewrite wordToN_combine
+    | [|- context[@wordToN _ (@zext _ _ _)] ] =>
+      rewrite wordToN_zext
+    | [|- context[@wordToN _ (@wones _)] ] =>
+      rewrite wordToN_wones
+    end.
+
+  Lemma break_spec: forall (m n: nat) (x: word n) low high,
+      (low, high) = break m x
+    -> &x = (&high * Npow2 m + &low)%N.
+  Proof.
+    intros m n x low high H.
+    unfold break in H.
+    destruct (le_dec m n).
+
+    - inversion H; subst; clear H.
+      propagate_wordToN.
+      rewrite N.land_ones.
+      rewrite N.shiftr_div_pow2.
+      replace (n - (n - m)) with m by omega.
+      rewrite N.mul_comm.
+      rewrite Npow2_N.
+      rewrite <- (N.div_mod' (& x) (2 ^ (N.of_nat m))%N).
+      reflexivity.
+
+    - inversion H; subst; clear H.
+      propagate_wordToN; simpl; nomega.
+  Qed.
+
+  Lemma extend_bound: forall k n (p: (k <= n)%nat) (w: word k),
+    (& (extend p w) < Npow2 k)%N.
+  Proof.
+    intros.
+    propagate_wordToN.
+    apply word_size_bound.
+  Qed.
+
+  Lemma mask_spec : forall (n: nat) (x: word n) m,
+    & (mask (N.to_nat m) x) = (N.land (& x) (N.ones m)).
+  Proof.
+    intros; unfold mask.
+    destruct (le_dec (N.to_nat m) n).
+
+    - propagate_wordToN.
+      rewrite N2Nat.id.
+      reflexivity.
+    
+    - rewrite N.land_ones.
+      rewrite N.mod_small; try reflexivity.
+      rewrite <- (N2Nat.id m).
+      rewrite <- Npow2_N.
+      apply (N.lt_le_trans _ (Npow2 n) _); try apply word_size_bound.
+      apply Npow2_ordered.
+      omega.
+  Qed.
+
+  Lemma mask_bound : forall (n: nat) (x: word n) m,
+    (& (mask m x) < Npow2 m)%N.
+  Proof.
+    intros; unfold mask.
+    destruct (le_dec m n).
+
+    - apply extend_bound.
+
+    - apply (N.lt_le_trans _ (Npow2 n) _); try apply word_size_bound.
+      apply Npow2_ordered.
+      omega.
+  Qed.
+
+End SpecialFunctions.
+
+Section TopLevel.
+  Local Open Scope nword_scope.
+
+  Coercion ind : bool >-> N.
+
+  Lemma wordize_plus: forall {n} (x y: word n),
+      (&x + &y < Npow2 n)%N
+    -> (&x + &y)%N = & (x ^+ y).
+  Proof.
+    intros n x y H.
+    pose proof (word_size_bound x) as Hbx.
+    pose proof (word_size_bound y) as Hby.
+
+    unfold wplus, wordBin.
+    rewrite wordToN_NToWord; intuition.
+  Qed.
+
+  Lemma wordize_awc: forall {n} (x y: word n) (c: bool),
+      (&x + &y + c < Npow2 n)%N
+    -> (&x + &y + c)%N = &(addWithCarry x y c).
+  Proof.
+    intros n x y c H.
+    unfold wplus, wordBin, addWithCarry.
+    destruct c; simpl in *.
+
+    - replace 1%N with (wordToN (natToWord n 1)) in * by (
+        rewrite wordToN_nat;
+        rewrite wordToNat_natToWord_idempotent;
+        nomega).
+
+      rewrite <- N.add_assoc.
+      rewrite wordize_plus; try nomega.
+      rewrite wordize_plus; try nomega.
+
+      + rewrite wplus_assoc.
+        reflexivity.
+
+      + apply (N.le_lt_trans _ (& x + & y + & natToWord n 1)%N _);
+          try assumption.
+        rewrite <- N.add_assoc.
+        apply N.add_le_mono.
+
+        * apply N.eq_le_incl; reflexivity.
+
+        * apply plus_le.
+
+    - rewrite wplus_comm.
+      rewrite wplus_unit.
+      rewrite N.add_0_r in *.
+      apply wordize_plus; assumption.
+  Qed.
+
+  Lemma wordize_mult: forall {n} (x y: word n),
+      (&x * &y < Npow2 n)%N
+    -> (&x * &y)%N = &(x ^* y).
+  Proof.
+    intros n x y H.
+    pose proof (word_size_bound x) as Hbx.
+    pose proof (word_size_bound y) as Hby.
+
+    unfold wmult, wordBin.
+    rewrite wordToN_NToWord; intuition.
+  Qed.
+
+  Lemma wordize_shiftr: forall {n} (x: word n) (k: nat),
+    (N.shiftr_nat (&x) k) = & (shiftr x k).
+  Proof.
+    intros n x k.
+    unfold shiftr, extend, high.
+    destruct (le_dec k n).
+
+    - repeat first [
+        rewrite wordToN_convS
+      | rewrite wordToN_zext
+      | rewrite wordToN_split2 ].
+      rewrite <- Nshiftr_equiv_nat.
+      reflexivity.
+
+    - rewrite (wordToN_nat (wzero n)); unfold wzero.
+      destruct (Nat.eq_dec n O); subst.
+
+      + rewrite (shatter_word_0 x); simpl; intuition.
+        rewrite <- Nshiftr_equiv_nat.
+        rewrite N.shiftr_0_l.
+        reflexivity.
+
+      + rewrite wordToNat_natToWord_idempotent;
+          try nomega.
+
+        * pose proof (word_size_bound x).
+          rewrite <- Nshiftr_equiv_nat.
+          rewrite N.shiftr_eq_0_iff.
+          destruct (N.eq_dec (&x) 0%N) as [E|E];
+            try rewrite E in *;
+            try abstract (left; reflexivity).
+
+          right; split; try nomega.
+          apply (N.le_lt_trans _ (N.log2 (Npow2 n)) _). {
+            apply N.log2_le_mono.
+            apply N.lt_le_incl.
+            assumption.
+          }
+
+          rewrite Npow2_N.
+          rewrite N.log2_pow2; try nomega.
+          apply N_ge_0.
+
+        * simpl; apply Npow2_gt0.
+  Qed.
+
+  Lemma conv_mask: forall {n} (x: word n) (k: nat),
+    (k <= n)%nat ->
+    mask k x = x ^& (NToWord _ (N.ones (N.of_nat k))).
+  Proof.
+    intros n x k H.
+    apply NToWord_equal.
+
+    rewrite <- (Nat2N.id k).
+    rewrite mask_spec.
+    apply N.bits_inj_iff; unfold N.eqf; intro m.
+    rewrite N.land_spec.
+    repeat rewrite wordToN_testbit.
+    rewrite <- (N2Nat.id m).
+    rewrite <- wordToN_wones.
+    repeat rewrite wordToN_testbit.
+    repeat rewrite N2Nat.id.
+    rewrite <- wordToN_wones.
+
+    assert (forall n (a b: word n) k,
+        wbit (a ^& b) k = andb (wbit a k) (wbit b k)) as Hwand. {
+      intros n0 a b.
+      induction n0 as [|n1];
+        shatter a; shatter b;
+        simpl; try reflexivity.
+
+      intro k0; induction k0 as [|k0];
+        simpl; try reflexivity.
+
+      fold wand.
+      rewrite IHn1.
+      reflexivity.
+    }
+
+    rewrite Hwand; clear Hwand.
+    induction (wbit x (N.to_nat m));
+      repeat rewrite andb_false_l;
+      repeat rewrite andb_true_l;
+      try reflexivity.
+
+    repeat rewrite <- wordToN_testbit.
+    rewrite wordToN_NToWord; try reflexivity.
+    apply (N.lt_le_trans _ (Npow2 k) _).
+
+    + apply word_size_bound.
+
+    + apply Npow2_ordered.
+      omega.
+  Qed.
+
+  Close Scope nword_scope.
+End TopLevel.
+
